fix bug in performance predicates where ProcEpAck was omitted from transition to PrepSync after electingFollowers becomes a quorum. Fix associated proofs. Halfway through Sync_Leader_PreQuorum_Invariant_helper lemma

ironfleet/src/Dafny/Distributed/Protocol/ZooKeeper/PerformamceProof/PerformancePredicates.dfy
@@ -273,6 +273,7 @@ function Sync_Message_ts_Formula(f:int, serial:nat) : Timestamp
     requires f >= 1;
 {
     AckEpoch_Message_PreQuorum_ts_Formula(f, f-1)
+    + ProcEpAck * f
     + PreSync * f    // max possible PrepSyncs done before I was sent
     + Sync * serial  // max possible NewLeader sent before I was sent
     + Sync * (serial + 1)  // I am the (serial + 1)-th sync message sent
@@ -284,6 +285,7 @@ function NewLeader_Message_ts_Formula(f:int, serial:nat) : Timestamp
     requires f >= 1;
 {
     AckEpoch_Message_PreQuorum_ts_Formula(f, f-1)
+    + ProcEpAck * f
     + PreSync * f    // max possible PrepSyncs done before I was sent
     + Sync * f  // max possible Syncs sent before I was sent
     + Sync * (serial + 1)  // I am the (serial + 1)-th NL message sent
@@ -334,6 +336,7 @@ function ProcessAck_PreQuorum_ts_Formula(f:int, n:int, l:TQuorumPeer) : Timestam
     var ackSet := l.v.leader.globals.ackSet;
     if |ackSet| <= 1 then 
         AckEpoch_Message_PreQuorum_ts_Formula(f, f-1)
+        + ProcEpAck * l.v.leader.globals.procEpCount 
         + PreSync * l.v.leader.globals.prepCount    // num of PrepSyncs done
         + Sync * l.v.leader.globals.nextSerialSync   // Only sync, never syncSnap
         + Sync * l.v.leader.globals.nextSerialNL   // Only sync, never syncSnap
@@ -394,7 +397,7 @@ predicate Sync_Leader_PreQuorum_Invariant(tls:TLS_State)
 {
     var n := |tls.config|;
     var leaderTQP := tls.t_servers[tls.config[0]];
-    !IsQuorum(n, leaderTQP.v.leader.globals.ackSet)
+    && !IsQuorum(n, leaderTQP.v.leader.globals.ackSet)
     ==> 
     && leaderTQP.ts <= ProcessAck_PreQuorum_ts_Formula(tls.f, n, leaderTQP)
     && leaderTQP.dts <= ProcessAck_PreQuorum_dts_Formula(tls.f, n, leaderTQP)
